---
size: double
---
# Trigonometric Functions

::trigonometricfunctions

<!--
visual:
:::
<LawOfTangents />
:::

visual:
:::
TrigonometricFunctions
:::

## [[Angles]]

Given a triangle $ABC$ where:

$$
\begin{array}{rl}
	\BA
		a &= BC \\
		b &= AC \\
		c &= AB 
	\EA
	&
	\BA
		\alpha &= \angle BC \\
		\beta &= \angle AC \\
		\zeta &= \angle AB
	\EA
\end{array}
$$

## Low of sines

$$
	\frac{\sin \alpha}{a} =
	\frac{\sin \beta}{b} =
	\frac{\sin \zeta}{c}
$$

## Low of cosines

$$
	c^2 = a^2 + b^2 - 2ab \cos \zeta
$$

## Low of tangents

$$
	\frac{a + b}{a - b} = 
	\frac{
		\tan(\frac{\alpha + \beta}{2})
	}{
		\tan(\frac{\alpha - \beta}{2})
	}
$$

## Addition

$$
\BA
	\cos (\alpha + \beta) & = 
	\cos \alpha \cos \beta - \sin \alpha \sin \beta \\
	\cos (\alpha - \beta) & = 
	\cos \alpha \cos \beta + \sin \alpha \sin \beta \\
	\sin (\alpha + \beta) & = 
	\sin \alpha \cos \beta + \cos \alpha \sin \beta \\
	\sin (\alpha - \beta) & = 
	\sin \alpha \cos \beta - \cos \alpha \sin \beta \\
	\tg (\alpha + \beta) & = 
	\frac{\tg \alpha + \tg \beta}{1 - \tg \alpha \tg \beta} \\
	\tg (\alpha - \beta) & = 
	\frac{\tg \alpha - \tg \beta}{1 + \tg \alpha \tg \beta} \\
	\ctg (\alpha + \beta) & = 
	\frac{\ctg \alpha \ctg \beta - 1}{\ctg \alpha + \ctg \beta} \\
	\ctg (\alpha - \beta) & = 
	\frac{\ctg \alpha \ctg \beta + 1}{\ctg \beta - \ctg \alpha}
\EA
$$

## Double angle

$$
\BA
	\sin 2 \alpha & = 2 \sin \alpha \cos \alpha \\
	\cos 2 \alpha & = 
	\cos^2 \alpha - \sin^2 \alpha =
	1 - 2 \sin^2 \alpha =
	2 \cos^2 \alpha - 1 \\
\EA
$$
-->
